cava/monad-examples/ExamplesSV.hs
@@ -18,6 +18,7 @@ module Main where
 
 import Cava2SystemVerilog
 import NandGate
+import Mux2_1
 import FullAdder
 import UnsignedAdderExamples
 import AdderTree
@@ -29,6 +30,8 @@ main = do writeSystemVerilog nand2Netlist
           writeTestBench pipelinedNAND_tb
           writeSystemVerilog loopedNANDNetlist
           writeTestBench loopedNAND_tb
+          writeSystemVerilog mux2_1Netlist
+          writeTestBench mux2_1_tb
           writeSystemVerilog adder4Netlist
           writeTestBench adder4_tb
           writeSystemVerilog adder8_3inputNetlist
