cava/monad-examples/Mux2_1.v
@@ -1,0 +1,66 @@
+(* Copyright 2020 The Project Oak Authors                                   *)
+(*                                                                          *)
+(* Licensed under the Apache License, Version 2.0 (the "License")           *)
+(* you may not use this file except in compliance with the License.         *)
+(* You may obtain a copy of the License at                                  *)
+(*                                                                          *)
+(*     http://www.apache.org/licenses/LICENSE-2.0                           *)
+(*                                                                          *)
+(* Unless required by applicable law or agreed to in writing, software      *)
+(* distributed under the License is distributed on an "AS IS" BASIS,        *)
+(* WITHOUT WARRANTIES OR CONDITIONS OF ANY KIND, either express or implied. *)
+(* See the License for the specific language governing permissions and      *)
+(* limitations under the License.                                           *)
+(****************************************************************************)
+
+Require Import Program.Basics.
+From Coq Require Import Bool.Bool.
+From Coq Require Import Ascii String.
+From Coq Require Import Lists.List.
+Import ListNotations.
+
+Require Import ExtLib.Structures.Monads.
+
+Require Import Cava.Monad.Cava.
+Require Import Cava.Netlist.
+
+Local Open Scope list_scope.
+Local Open Scope monad_scope.
+Local Open Scope string_scope.
+
+Definition mux2_1 {m bit} `{Cava m bit} '(sel, (a, b)) : m bit :=
+  o <- indexBitArray [a; b] [sel] ;;
+  ret o.
+
+Example m1: combinational (mux2_1 (false, (false, true))) = false.
+Proof. reflexivity. Qed.
+
+Example m2: combinational (mux2_1 (false, (true, false))) = true.
+Proof. reflexivity. Qed.
+
+Example m3: combinational (mux2_1 (true, (false, true))) = true.
+Proof. reflexivity. Qed.
+
+Example m4: combinational (mux2_1 (true, (true, false))) = false.
+Proof. reflexivity. Qed.
+
+Definition mux2_1_Interface
+  := mkCircuitInterface "mux2_1"
+     (Tuple2 (One ("sel", Bit)) (Tuple2 (One ("i0", Bit)) (One ("i1", Bit))))
+     (One ("o", Bit))
+     [].
+
+Definition mux2_1Netlist := makeNetlist mux2_1_Interface mux2_1.
+
+Definition mux2_1_tb_inputs :=
+  [(false, (false, true));
+   (false, (true, false));
+   (true, (false, true));
+    (true, (true, false))].
+
+Definition mux2_1_tb_xpected_outputs
+  := map (fun i => combinational (mux2_1 i)) mux2_1_tb_inputs.
+
+Definition mux2_1_tb
+  := testBench "mux2_1_tb" mux2_1_Interface
+     mux2_1_tb_inputs mux2_1_tb_xpected_outputs.  
